LeanFomega/Kinding/Rename.lean
@@ -1,0 +1,22 @@
+
+import LeanFomega.Typing
+open LeanSubst
+
+namespace LeanFomega
+
+structure KindingRen (r : Ren) (Δ1 Δ2 : List Kind) where
+  act : ∀ {x T}, Δ1[x]? = some T -> Δ2[r.act x]? = some T
+
+notation:35 Γ:35 " -⟨" r "⟩> " Δ:35 => KindingRen r Γ Δ
+
+theorem KindingRen.lift A : Δ1 -⟨r⟩> Δ2 -> A::Δ1 -⟨r.lift⟩> A::Δ2 := sorry
+
+theorem KindingRen.id X : X -⟨.id⟩> X := sorry
+
+theorem KindingRen.succ : X -⟨Ren.add 1⟩> A::X := sorry
+
+theorem KindingRen.comp : A -⟨r1⟩> B -> B -⟨r2⟩> C -> A -⟨r1 ∘ r2⟩> C := sorry
+
+def Kinding.rename (m : Δ1 -⟨r⟩> Δ2) : Δ1 ⊢ₖ A : K -> Δ2 ⊢ₖ A⟨r⟩ : K := sorry
+
+end LeanFomega
