LeanFomega/Kinding/StrongNorm.lean
@@ -1,0 +1,90 @@
+
+import LeanSubst
+import LeanFomega.Typing
+import LeanFomega.Kinding.Substitute
+open LeanSubst
+
+namespace LeanFomega
+
+def KSet := List Kind -> Ty -> Kind -> Prop
+def KSet.empty : KSet := λ _ _ _ => False
+def KRed := List Kind -> Ty -> Ty -> Prop
+
+def ℛₖ (S : List Kind -> Ty -> Prop) : List Kind -> Ty -> Prop
+| Δ1, t => ∀ {r Δ2}, Δ1 -⟨r⟩> Δ2 -> S Δ2 t[r]
+
+mutual
+  inductive Kinding.SnNor : (List Kind -> Ty -> Prop) -> KSet
+  | lam :
+    ℛₖ S1 Δ (λ[A] t) ->
+    SnNor S2 (A::Δ) t B ->
+    SnNor S1 Δ (λ[A] t) (A -:> B)
+  | all :
+    SnNor S (A::Δ) t ★ ->
+    SnNor S Δ (∀[A] t) ★
+  | arrow :
+    SnNor S Δ A ★ ->
+    SnNor S Δ B ★ ->
+    SnNor S Δ (A -:> B) ★
+  | neu :
+    SnNeu S Δ A K ->
+    SnNor S Δ A K
+  | red :
+    SnRed Δ S A A' ->
+    SnNor Δ S A' K ->
+    SnNor Δ S A K
+
+  inductive Kinding.SnNeu : (List Kind -> Ty -> Prop) -> KSet
+  | var :
+    Δ[x]? = some K ->
+    SnNeu S Δ t#x K
+  | app :
+    SnNeu S1 Δ f (A -:> B) ->
+    SnNor S2 Δ a A ->
+    SnNeu S3 Δ (f • a) B
+
+  inductive Kinding.SnRed : (List Kind -> Ty -> Prop) -> KRed
+  | beta :
+    SnNor S1 Δ t A ->
+    SnRed S2 Δ ((λ[A] b) • t) b[su t::+0]
+  | app :
+    SnRed S1 Δ f f' ->
+    SnRed S2 Δ (f • a) (f' • a)
+end
+
+mutual
+  theorem Kinding.SnNor.rename (m : Δ1 -⟨r⟩> Δ2) : SnNor S Δ1 A K -> SnNor S Δ2 A[r] K := sorry
+
+  theorem Kinding.SnNeu.rename (m : Δ1 -⟨r⟩> Δ2) : SnNeu S Δ1 A K -> SnNeu S Δ2 A[r] K := sorry
+
+  theorem Kinding.SnRed.rename (m : Δ1 -⟨r⟩> Δ2) : SnRed S Δ1 A B -> SnRed S Δ2 A[r] B[r] := sorry
+end
+
+@[simp]
+def 𝒱ₖ : Kind -> List Kind -> Ty -> Prop
+| A -:> B, Δ, λ[_] t => ∀ {a}, Kinding.SnNor (𝒱ₖ A) Δ a A -> Kinding.SnNor (𝒱ₖ B) Δ t[su a::+0] B
+| _, _, _ => False
+
+structure Kinding.SemSubst (Δ1 Δ2 : List Kind) (σ : Subst Ty) where
+  act : ∀ {i T}, Δ1[i]? = some T -> SnNor (𝒱ₖ T) Δ2 (σ.act i) T
+
+notation:35 Γ:35 " -⟦" σ "⟧> " Δ:35 => Kinding.SemSubst Γ Δ σ
+
+theorem Kinding.SemSubst.lift (m : Γ -⟦σ⟧> Δ) A : A::Γ -⟦σ.lift⟧> A::Δ := sorry
+
+theorem Kinding.SemSubst.compose (m1 : Γ -⟦σ⟧> Δ) (m2 : Δ -⟨r⟩> Ξ) : Γ -⟦σ ∘ r.to⟧> Ξ := sorry
+
+@[simp]
+def SemanticKinding (Δ1 : List Kind) (A : Ty) (K : Kind) :=
+  ∀ {σ Δ2}, Δ1 -⟦σ⟧> Δ2 -> Kinding.SnNor (𝒱ₖ K) Δ2 A[σ] K
+
+notation:170 Γ:170 " ⊨ₖ " t:170 " : " A:170 => SemanticKinding Γ t A
+
+theorem Kinding.fundamental : Δ ⊢ₖ A : K -> Δ ⊨ₖ A : K
+| var j, σ, Δ2, h => sorry
+| lam j, σ, Δ2, h => sorry
+| app j1 j2, σ, Δ2, h => sorry
+| all j, σ, Δ2, h => .all $ j.fundamental $ h.lift _
+| arrow j1 j2, σ, Δ2, h => .arrow (j1.fundamental h) (j2.fundamental h)
+
+end LeanFomega
