LeanFomega/Typing/Rename.lean
@@ -1,0 +1,27 @@
+
+import LeanFomega.Typing
+import LeanFomega.Kinding.Rename
+open LeanSubst
+
+namespace LeanFomega
+
+structure TypingRen (r : Ren) (Γ1 Γ2 : List Ty) where
+  act : ∀ {x T}, Γ1[x]? = some T -> Γ2[r.act x]? = some T
+
+notation:35 Γ:35 " -⟨" r "⟩> " Δ:35 => TypingRen r Γ Δ
+
+theorem TypingRen.lift {Γ1 Γ2 : List Ty} A : Γ1 -⟨r⟩> Γ2 -> A::Γ1 -⟨r.lift⟩> A::Γ2 := sorry
+
+theorem TypingRen.id (X : List Ty) : X -⟨.id⟩> X := sorry
+
+theorem TypingRen.succ {X : List Ty} : X -⟨Ren.add 1⟩> A::X := sorry
+
+theorem TypingRen.comp {A B C : List Ty} : A -⟨r1⟩> B -> B -⟨r2⟩> C -> A -⟨r1 ∘ r2⟩> C := sorry
+
+def Typing.rename_type {Δ1 Δ2 : List Kind} (m : Δ1 -⟨r⟩> Δ2)
+  : Δ1&Γ ⊢ t : A -> Δ2&Γ⟨.add 1⟩ ⊢ t : A⟨r⟩ := sorry
+
+def Typing.rename {Γ1 Γ2 : List Ty} (m : Γ1 -⟨r⟩> Γ2)
+  : Δ&Γ1 ⊢ t : A -> Δ&Γ2 ⊢ t⟨r⟩ : A := sorry
+
+end LeanFomega
